theories/examples/susp_correctness/correctness.v
@@ -690,9 +690,10 @@ Section proof.
 
     - iMod (na_inv_acc with "Hinv_unfill Htok") as "(>Hinvo & Htok & Hclose_inv)"; try solve_ndisj.
       iDestruct "Hinvo" as "[(%& Hlb & Hlr & Hbrproph)|
-              (%&%&%&%& Hlb & Hlr & Hbrproph & #Hpfrag & #Hgetvisit)]";
+              (%&%&%&%& Hlb & Hlr & Hbrproph & #Hlbpfrag' & #Hgetvisit)]";
         wp_load; last first.
       + iDestruct ("Hgetvisit" with "Hst") as "[Hst #Hvisit]".
+        iDestruct (lg_mapg_p_agree with "Hlbpfrag Hlbpfrag'") as "(% & _ & _)".
         destruct r.
         * iMod ("Hclose_inv" with "[$Htok Hlb Hlr Hbrproph]") as "Htok".
           { iNext. iRight. iFrame "∗ #". eauto. }
@@ -785,7 +786,7 @@ Section proof.
             iIntros "Hst". by iFrame. }
 
           iDestruct (id_ctr_frag_agree with "Hvmauth Hid") as "->".
-          iMod (id_ctr_frag_alloc _ _ _ susp with "Hvmauth Hid") as "(Hvmauth & Hid & Hidtok & Hvfrag)".
+          iMod (id_ctr_frag_alloc _ _ _ susp with "Hvmauth Hid") as "(Hvmauth & Hid & Hidtok & #Hvfrag)".
 
           iSimpl in "Hv". v_pures. v_bind (v_count _).
           iDestruct "Hc" as "(Hcap & % & Hc & Hagg)".
@@ -795,10 +796,254 @@ Section proof.
           iMod (v_finish_spec with "Htab Hv") as (v_finish) "[Hvfinish Hv] /=".
           v_pures; try solve_vals_compare_safe.
 
+          set (vm' := set_fold (λ (γ : gname) (m0 : state_mapg_type), <[γ:=pending_val]> m0) vm γl).
+          set (pn' := definitions.sum_list lpn + size γl).
+          set (cntr' := S cntr).
+          simplify_eq.
+          assert (pn' = size γl + definitions.sum_list lpn) as <- by lia.
+
+          iAssert (
+            |={⊤}=>
+              seq_tok ⊤ ∗
+              auth_v cntr (InjRV #susp) s ∗
+              ((∃ vm'',
+                  ⌜vm'' = (<[ γ0 := done_val cntr ]>vm')⌝ ∗
+                  visited_mapg_auth vm'' pn' cntr') ∨
+              (visit_finished γ0 ∗
+                visited_mapg_auth vm' pn' cntr')))%I
+            with "[Htok Hintr Hidtok Hvmauth]"
+          as ">(Htok & Hauthv & Hvmauth')".
+          { iMod (na_inv_acc with "Hinv_authv Htok") as "(>Hinvo & Htok & Hclose)";
+              try solve_ndisj.
+            iDestruct "Hinvo" as "[Hinv_1|Hinv_2]".
+            - iDestruct "Hinv_1" as "(%s1&% & (%&%&%&%& Hsusp & #Hfilled & #Hlbvfrag' & #Hvisfin))".
+              destruct! H6. simplify_eq.
+              iDestruct (lg_mapg_agree with "Hlbvfrag Hlbvfrag'") as "(<- & _ & _)".
+              iPoseProof (id_token_unused with "Hvmauth Hidtok") as "(%Hidunused & $ & Hidtok)".
+              iFrame "Hmauth Hbigsep". iModIntro.
+              iExists _. iSplit; eauto.
+              iSplitR.
+              { iModIntro. iIntros (gpid gsusp gγ Hgpid_lt) "H1 H2 H3".
+                iDestruct ("Hnmspc" with "[] H1 H2 H3") as "%Hsubset".
+                { iPureIntro. lia. }
+                iPoseProof (pval_snapshot_neq with "Hpvuneq H1") as "%Hneq";
+                  try lia.
+                iPureIntro.
+                assert ((↑ver_susp_n gsusp : coPset) ## ↑ver_susp_n susp) as Hdisj.
+                { apply ndot_ne_disjoint. by intros ->. }
+                set_solver. }
+              iSplitR "Hvisinv".
+              { iRight. rewrite H10.
+                iFrame "Hgpfrag Hidtok Hxinv Hxlbfrag Htok".
+                repeat (iSplit; eauto). iSplitR. { by iIntros. }
+                repeat (iSplit; eauto).
+                iSplitR "Hclose_inv".
+                { iLeft. iFrame "∗ #". iExists s1.
+                  repeat (iSplit; eauto). 
+                  unfold filled_string in *. 
+                  unfold simple_string in *. 
+                  simplify_eq. by rewrite H8. }
+                iFrame. }
+
+                (* iSplit. { iPureIntro. admit. }
+                admit. } *)
+
+              iRight. iApply (big_sepM_mono with "Hvisinv").
+              iIntros (k x' Hkx) "Hvis".
+              iIntros (id_inner Heq').
+              assert (id_inner ≠ pid).
+              { intros ->. specialize (Hidunused k). simplify_eq. }
+              rewrite (lookup_delete_ne); last first.
+              { intros ?. simplify_eq. }
+              by iApply "Hvis".
+
+            - iDestruct "Hinv_2" as "(%&%&%&%&%&%&%& Hxcap & Hxunfill & Hxmfrag & %Hxmsub & Hxsusp & Hxproph)".
+
+              iPoseProof (mapg_auth_alive with "Hmauth Hxmfrag") as (yx) "%Hxin".
+              destruct Hxin as [(?&Hxin&?)%Some_equiv_eq ?].
+              edestruct (mapg_alive_lookup_Cinl _ _ _ yx Hxin) as (yx' & Halive & Hyyx'); first done.
+              clear Hxin. rename Halive into Hxin.
+
+              iDestruct (big_sepM_lookup_acc _ (mapg_alive (<[pid:=csum.Cinr (to_agree ())]> m')) pid0 _ Hxin with "Hbigsep") as "[Hms Hbigsep]".
+              iDestruct "Hms" as (ctr ????????[Hxcgt [Hxin' ?]]) 
+                  "(Hlc & Hxxser & Hxxserspec & Hxxauth & Hxxc & Hxxfin)".
+              
+              simplify_eq.
+              iMod (visit_update_finished with "Hvmauth Hxvisdone Hintr Hxlbfrag
+                Hxsusp Hxxc") as "(#Hxvisfin & Hintr & Hvmauth & Hxxc & Hxsusp)".
+              { assert (x2 = pv0) as ->.
+                { rewrite Hyyx' in H11. rewrite H11 in H10. simpl in H10.
+                  fold_leibniz. by apply (inj to_agree) in H10. }
+                exact Hxmsub. }
+
+              iEval (rewrite visited_map_update_finished_rewrite) in "Hvmauth".
+              iPoseProof ("Hgetidtok" with "Hxvisfin") as "Hidtok".
+              iPoseProof (id_token_unused with "Hvmauth Hidtok")
+                as "(%Hidunused & Hvmauth & Hidtok)".
+              iAssert (visit_finished _ -∗ id_token pid)%I with "[Hidtok]"
+                as "Hgetidtok".
+              { iIntros "_". iExact "Hidtok". }
+
+              iFrame "Hmauth".
+              iPoseProof ("Hbigsep" with 
+                  "[$Hlc $Hxxser $Hxxserspec $Hxxauth $Hxxc $Hxxfin]") as "$".
+              { eauto. }
+
+              iExists _. iSplitR; eauto.
+              iSplitR.
+              { do 2 iModIntro. iIntros (gpid gsusp gγ Hgpid_lt) "H1 H2 H3".
+                iDestruct ("Hnmspc" with "[] H1 H2 H3") as "%Hsubset".
+                { iPureIntro. lia. }
+                iPoseProof (pval_snapshot_neq with "Hpvuneq H1") as "%Hneq";
+                  try lia.
+                iPureIntro.
+                assert ((↑ver_susp_n gsusp : coPset) ## ↑ver_susp_n susp) as Hdisj.
+                { apply ndot_ne_disjoint. by intros ->. }
+                set_solver. }
+              iSplitR "Hvisinv Hvmauth".
+              { iRight. iFrame "∗ #".
+                iModIntro. repeat (iSplit; eauto).
+                iRight. iFrame "∗ #". eauto. }
+              { iModIntro. iLeft. iExists _, _.
+                iSplit; first done.
+                iFrame "Hvmauth".
+                rewrite -insert_delete_insert.
+                iApply big_sepM_insert_2.
+                - iIntros (id_x [=]).
+                - iPoseProof (big_sepM_subseteq with "Hvisinv") as "Hvisinv";
+                    first apply delete_subseteq.
+                  iApply (big_sepM_mono with "Hvisinv").
+                  iIntros (k vk Hkv) "Hv".
+                  iIntros (id_x ->).
+                  apply lookup_delete_Some in Hkv as [Hkne Hkv].
+                  iSpecialize ("Hv" $! id_x eq_refl).
+                  iDestruct "Hv" as (v') "%Hmlookup".
+                  iExists v'. iPureIntro.
+                  rewrite lookup_delete_ne; first done.
+                  intros Hpideq. assert (id_x = pid) by (by simplify_eq).
+                  subst id_x.
+                  specialize (Hidunused k).
+                  rewrite lookup_insert_ne in Hidunused; last done.
+                  by apply Hidunused. } }
+
           case_bool_decide; simplify_eq; v_pures.
           -- v_bind (v_finish _).
             assert (size γl = 0) as -> by lia.
             iDestruct "Hmauth" as "[[% Hmauth]|[% Hmauth]]"; try lia.
+
+            { iDestruct "Hinvo" as "[Hinv_1|Hinv_2]".
+              - iDestruct "Hinv_1" as "(%s1&% & (%&%&%&%& Hsusp & #Hfilled & #Hlbvfrag' & #Hvisfin))".
+                destruct! H7. simplify_eq.
+                iPoseProof ("Hgetidtok" with "Hvisfin") as "Hidtok".
+                iPoseProof (id_token_unused with "Hvmauth Hidtok") as "(%Hidunused & $ & Hidtok)".
+                iFrame "Hmauth Hbigsep". iModIntro.
+                iExists _. iSplit; eauto.
+                iSplitR.
+                { iModIntro. iIntros (gpid gsusp gγ Hgpid_lt) "H1 H2 H3".
+                  iDestruct ("Hnmspc" with "[] H1 H2 H3") as "%Hsubset".
+                  { iPureIntro. lia. }
+                  iPoseProof (pval_snapshot_neq with "Hpvuneq H1") as "%Hneq";
+                    try lia.
+                  iPureIntro.
+                  assert ((↑ver_susp_n gsusp : coPset) ## ↑ver_susp_n susp) as Hdisj.
+                  { apply ndot_ne_disjoint. by intros ->. }
+                  set_solver. }
+                iSplitR "Hvisinv".
+                { iRight. rewrite H10.
+                  iFrame "Hgpfrag Hidtok Hxinv Hxlbfrag Htok".
+                  repeat (iSplit; eauto). iSplitR. { by iIntros. }
+                  repeat (iSplit; eauto).
+                  iSplitR "Hclose_inv".
+                  { iLeft. iFrame "∗ #". iExists s1.
+                    repeat (iSplit; eauto). 
+                    unfold filled_string in *. 
+                    unfold simple_string in *. 
+                    simplify_eq. by rewrite H8. }
+                  iFrame. }
+
+                  (* iSplit. { iPureIntro. admit. }
+                  admit. } *)
+
+                iRight. iApply (big_sepM_mono with "Hvisinv").
+                iIntros (k x' Hkx) "Hvis".
+                iIntros (id_inner Heq').
+                assert (id_inner ≠ pid).
+                { intros ->. specialize (Hidunused k). simplify_eq. }
+                rewrite (lookup_delete_ne); last first.
+                { intros ?. simplify_eq. }
+                by iApply "Hvis".
+
+              - iDestruct "Hinv_2" as "(%&%&%&%&%&%&%& Hxcap & Hxunfill & Hxmfrag & %Hxmsub & Hxsusp & Hxproph)".
+
+                iPoseProof (mapg_auth_alive with "Hmauth Hxmfrag") as (yx) "%Hxin".
+                destruct Hxin as [(?&Hxin&?)%Some_equiv_eq ?].
+                edestruct (mapg_alive_lookup_Cinl _ _ _ yx Hxin) as (yx' & Halive & Hyyx'); first done.
+                clear Hxin. rename Halive into Hxin.
+
+                iDestruct (big_sepM_lookup_acc _ (mapg_alive (<[pid:=csum.Cinr (to_agree ())]> m')) pid0 _ Hxin with "Hbigsep") as "[Hms Hbigsep]".
+                iDestruct "Hms" as (ctr ????????[Hxcgt [Hxin' ?]]) 
+                    "(Hlc & Hxxser & Hxxserspec & Hxxauth & Hxxc & Hxxfin)".
+                
+                simplify_eq.
+                iMod (visit_update_finished with "Hvmauth Hxvisdone Hintr Hxlbfrag
+                  Hxsusp Hxxc") as "(#Hxvisfin & Hintr & Hvmauth & Hxxc & Hxsusp)".
+                { assert (x2 = pv0) as ->.
+                  { rewrite Hyyx' in H11. rewrite H11 in H10. simpl in H10.
+                    fold_leibniz. by apply (inj to_agree) in H10. }
+                  exact Hxmsub. }
+
+                iEval (rewrite visited_map_update_finished_rewrite) in "Hvmauth".
+                iPoseProof ("Hgetidtok" with "Hxvisfin") as "Hidtok".
+                iPoseProof (id_token_unused with "Hvmauth Hidtok")
+                  as "(%Hidunused & Hvmauth & Hidtok)".
+                iAssert (visit_finished _ -∗ id_token pid)%I with "[Hidtok]"
+                  as "Hgetidtok".
+                { iIntros "_". iExact "Hidtok". }
+
+                iFrame "Hmauth".
+                iPoseProof ("Hbigsep" with 
+                    "[$Hlc $Hxxser $Hxxserspec $Hxxauth $Hxxc $Hxxfin]") as "$".
+                { eauto. }
+
+                iExists _. iSplitR; eauto.
+                iSplitR.
+                { do 2 iModIntro. iIntros (gpid gsusp gγ Hgpid_lt) "H1 H2 H3".
+                  iDestruct ("Hnmspc" with "[] H1 H2 H3") as "%Hsubset".
+                  { iPureIntro. lia. }
+                  iPoseProof (pval_snapshot_neq with "Hpvuneq H1") as "%Hneq";
+                    try lia.
+                  iPureIntro.
+                  assert ((↑ver_susp_n gsusp : coPset) ## ↑ver_susp_n susp) as Hdisj.
+                  { apply ndot_ne_disjoint. by intros ->. }
+                  set_solver. }
+                iSplitR "Hvisinv Hvmauth".
+                { iRight. iFrame "∗ #".
+                  iModIntro. repeat (iSplit; eauto).
+                  iRight. iFrame "∗ #". eauto. }
+                { iModIntro. iLeft. iExists _, _.
+                  iSplit; first done.
+                  iFrame "Hvmauth".
+                  rewrite -insert_delete_insert.
+                  iApply big_sepM_insert_2.
+                  - iIntros (id_x [=]).
+                  - iPoseProof (big_sepM_subseteq with "Hvisinv") as "Hvisinv";
+                      first apply delete_subseteq.
+                    iApply (big_sepM_mono with "Hvisinv").
+                    iIntros (k vk Hkv) "Hv".
+                    iIntros (id_x ->).
+                    apply lookup_delete_Some in Hkv as [Hkne Hkv].
+                    iSpecialize ("Hv" $! id_x eq_refl).
+                    iDestruct "Hv" as (v') "%Hmlookup".
+                    iExists v'. iPureIntro.
+                    rewrite lookup_delete_ne; first done.
+                    intros Hpideq. assert (id_x = pid) by (by simplify_eq).
+                    subst id_x.
+                    specialize (Hidunused k).
+                    rewrite lookup_insert_ne in Hidunused; last done.
+                    by apply Hidunused. } }
+
+            iDestruct "Hinvo" as "[Hinvo|Hinvo]".
+            {  }
 
             iMod ("Hclose_tab" with "[$Htabtok Hl Hbigsep Hmauth Hvmauth Hvisinv Hst']") as "Htabtok".
             { iNext. iLeft. iFrame "Hvmauth". iFrame "∗ %".
@@ -807,10 +1052,19 @@ Section proof.
               admit. (* rewrite set_fold as union. get disjointness.
                         apply big_sepM_union. *) }
 
-            iMod ("Hvfinish" $! ⊤ with "[] Htabtok Hlc Hvser Hvserspec Hc [Htok Hidtok Hintr Hvfrag]
+            iMod ("Hvfinish" $! ⊤ with "[] Htabtok Hlc Hvser Hvserspec Hc 
+                  [Htok Hidtok Hintr Hvfrag Hinvo Hclose]
                   Hst Hv") as "(Hv & Htabtok & Htok & Hst & Hintr) /=". 
             { iModIntro. iIntros (???) "_ _ _ _". set_solver. }
-            { iRight. iFrame "Hvfrag Hpvfrag Hpvuneq Hvisit Hinv_authv". } 
+            { iRight. iFrame "Hvfrag Hpvfrag Hpvuneq Hvisit Hinv_authv Hlbvfrag".
+              repeat (iSplit; eauto). { admit. }
+              iSplitL "Hidtok". { by iIntros "?". }
+              iSplit; eauto.
+              iFrame.
+
+              iSplitL "Hintr Hinvo".
+              { iLeft.  }
+               } 
             
             v_pures. v_bind (list_tail _).
             iMod (gwp_list_tail ⊤ _ (s_real :: _) () (λ v, ⌜is_proof _ ps2⌝)%I
